src/Analysis/Instances/Product/Ctx/Int_Ctx_None_Sound.thy
@@ -444,7 +444,7 @@ theorem ictx_activation_collect_sound:
      \<subseteq> gamma_state_lift (ictx_sg (Inl (v, ctx)))"
 proof (rule activation_collect_sound_gen[where sg = ictx_sg and gammaM = gamma_state_lift
         and enterc = "enterc_unit"
-        and startcontext = "()" and S = "cinit_stores gs" and g = "compile_prog Pi ps mnm main" and gs = gs])
+        and initial_ctx = "()" and S = "cinit_stores gs" and g = "compile_prog Pi ps mnm main" and gs = gs])
   \<comment> \<open>ENTRY_G\<close>
   fix s assume "s \<in> cinit_stores gs"
   hence "s \<in> gamma_state_lift (map_lift (fun_of_resolved_st_q_for gs) (Lifted cinit_int_dom_st))"
